fix(typing): pattern fragment in unification removed. from which arises various fixes and cleanup

examples/emoji.tig.lisp
@@ -22,7 +22,7 @@ let foo : List Bool × List String =
     fun x : ∀α, List α → List α =>
       ⟨x (Cons@Bool 😋 (Cons@Bool 😱 Nil@Bool)),
        x (Cons@String "😋" (Cons@String "😱" Nil@String))⟩
-  in f reverse@?sk.16
+  in f reverse@?m.16
 ;; == Runtime ==
 (load "runtime.lisp")
 
