examples/let-gen.tig.lisp
@@ -1,0 +1,96 @@
+;; == System F IR ==
+
+let i_C_0 : C (Λa. a) = C@(Λa. a) Λ a₁. fun x : a₁ => x
+
+let f : ∀α β [C α], β → α β =
+  Λ α β. fun d_C_0 : C α => fun x : β => d_C_0[0, c]@α x
+and g : Int → Int =
+  let rd_C_0 : C (Λa. a) = i_C_0 in fun y : Int => rd_C_0[0, c]@(Λa. a) y
+
+let i_C_1 : C Box = C@Box Λ a. fun x : a => Mk@a x x
+
+let main' : ∀α [C α], α (Box Bool) =
+  Λ α. fun d_C_0 : C α => f@α@(Box Bool) d_C_0 (Mk@Bool true false)
+
+let main : Box (Box Bool) = let rd_C_0 : C Box = i_C_1 in main'@Box rd_C_0
+;; == Runtime ==
+(load "runtime.lisp")
+
+;; == Linked Lisp Source ==
+(load "ffi.lisp")
+
+;; == Common Lisp ==
+
+; Prelude
+(declaim (optimize (speed 3) (safety 0) (debug 0)))
+(load "runtime.lisp")
+(defstruct (clos (:constructor %clos (fn arity)))
+  (fn #'identity :type function)
+  (arity 0 :type fixnum))
+(defun %apply-slow (c args)
+  (declare (type list args))
+  (let ((n (length args)) (k (clos-arity c)))
+    (cond
+      ((= n k) (apply (clos-fn c) args))
+      ((< n k) (%clos (lambda (&rest more)
+                        (apply (clos-fn c)
+                               (append args more)))
+                      (- k n)))
+      (t (%apply-slow (apply (clos-fn c)
+                             (subseq args 0 k))
+                      (nthcdr k args))))))
+
+
+; struct
+(defstruct (|Box| (:conc-name |Box/|) (:constructor nil) (:predicate nil))
+  (|tag| 0 :type (unsigned-byte 8)))
+
+(defstruct (|c/Mk| (:include |Box| (|tag| 0))
+  (:conc-name |Mk/|)
+  (:constructor |mk/Mk| (|f0| |f1|))
+  (:predicate |Mk?|))
+  (|f0| nil)
+  (|f1| nil))
+
+; gapply
+(defun gapply1 (c a1)
+  (if (eql (clos-arity c) 1)
+    (funcall (clos-fn c) a1)
+    (%apply-slow c (list a1))))
+
+; ftype
+(declaim (ftype (function (integer) integer) |fn-28|))
+
+(declaim (ftype (function (t) |Box|) |fn-29|))
+
+(declaim (type clos |g-11|))
+
+(declaim (type |Box| |main-25|))
+
+; body
+(defun |fn-27| (|x-4|)
+  |x-4|)
+
+(defun |fn-28| (|y-13|)
+  (|fn-27| |y-13|))
+
+(defun |fn-29| (|x-18|)
+  (|mk/Mk| |x-18| |x-18|))
+
+(defun |f-6| (|d_C_0-7| |x-8|)
+  (gapply1 |d_C_0-7| |x-8|))
+
+(defun |main'-21| (|d_C_0-22|)
+  (let* ((|con-23| (|mk/Mk| t nil))) (|f-6| |d_C_0-22| |con-23|)))
+
+(defparameter |i_C_0-2|
+  (%clos (function |fn-27|) 1))
+
+(defparameter |g-11|
+  (%clos (function |fn-28|) 1))
+
+(defparameter |i_C_1-16|
+  (%clos (function |fn-29|) 1))
+
+(defparameter |main-25|
+  (|main'-21| |i_C_1-16|))
