examples/recinst.tig.lisp
@@ -1,0 +1,136 @@
+;; == System F IR ==
+
+let (::) : ∀α, α → List α → List α = Λ α. Cons@α
+
+let i_Functor_0 : Functor List =
+  let rd_Functor_0 : Functor List = i_Functor_0
+  in Functor@List
+       Λ a b.
+         fun f : a → b =>
+           fun ?x₀ : List a =>
+             match ?x₀ with
+             | Nil => Nil@b
+             | Cons x xs => Cons@b (f x) (rd_Functor_0[0, fmap]@List f xs)
+
+let main : Int =
+  let rd_Functor_0 : Functor List = i_Functor_0
+  in let foldr : ∀α β, (α → β → β) → β → List α → β =
+       Λ α β.
+         rec fun foldr : (α → β → β) → β → List α → β =>
+           fun f : α → β → β =>
+             fun init : β =>
+               fun ?x₀ : List α =>
+                 match ?x₀ with
+                 | Nil => init
+                 | Cons x xs => f x (foldr f init xs)
+     in foldr@Int@Int fun ?x₀ : Int => fun ?x₁ : Int => add ?x₀ ?x₁ 0
+          (rd_Functor_0[0, fmap]@List fun ?x₀ : Int => add ?x₀ 1
+             (Cons@Int 1 (Cons@Int 2 (Cons@Int 3 Nil@Int))))
+;; == Runtime ==
+(load "runtime.lisp")
+
+;; == Linked Lisp Source ==
+(load "ffi.lisp")
+
+;; == Common Lisp ==
+
+; Prelude
+(declaim (optimize (speed 3) (safety 0) (debug 0)))
+(load "runtime.lisp")
+(defstruct (clos (:constructor %clos (fn arity)))
+  (fn #'identity :type function)
+  (arity 0 :type fixnum))
+(defun %apply-slow (c args)
+  (declare (type list args))
+  (let ((n (length args)) (k (clos-arity c)))
+    (cond
+      ((= n k) (apply (clos-fn c) args))
+      ((< n k) (%clos (lambda (&rest more)
+                        (apply (clos-fn c)
+                               (append args more)))
+                      (- k n)))
+      (t (%apply-slow (apply (clos-fn c)
+                             (subseq args 0 k))
+                      (nthcdr k args))))))
+
+
+; struct
+(defstruct (|List| (:conc-name |List/|) (:constructor nil) (:predicate nil))
+  (|tag| 0 :type (unsigned-byte 8)))
+
+(defstruct (|c/Nil| (:include |List| (|tag| 0))
+  (:conc-name |Nil/|)
+  (:constructor |mk/Nil| ())
+  (:predicate |Nil?|)))
+
+(defstruct (|c/Cons| (:include |List| (|tag| 1))
+  (:conc-name |Cons/|)
+  (:constructor |mk/Cons| (|f0| |f1|))
+  (:predicate |Cons?|))
+  (|f0| nil)
+  (|f1| nil))
+
+; gapply
+(defun gapply1 (c a1)
+  (if (eql (clos-arity c) 1)
+    (funcall (clos-fn c) a1)
+    (%apply-slow c (list a1))))
+
+(defun gapply2 (c a1 a2)
+  (if (eql (clos-arity c) 2)
+    (funcall (clos-fn c) a1 a2)
+    (%apply-slow c (list a1 a2))))
+
+; ftype
+(declaim (ftype (function (clos |List|) |List|) |fn-37|))
+
+(declaim (ftype (function (clos t |List|) t) |foldr-38|))
+
+(declaim (ftype (function (integer integer) integer) |fn-39|))
+
+(declaim (ftype (function (integer) integer) |fn-40|))
+
+(declaim (type integer |main-14|))
+
+; body
+(defun |fn-37| (|f-4| |?x₀-5|)
+  (case (|List/tag| |?x₀-5|)
+    (0
+      (|mk/Nil|))
+    (1
+      (let* ((|f-7| (|Cons/f0| |?x₀-5|))
+             (|f-8| (|Cons/f1| |?x₀-5|)))
+         (let* ((|app-9| (gapply1 |f-4| |f-7|))
+                (|app-11| (|fn-37| |f-4| |f-8|)))
+            (|mk/Cons| |app-9| |app-11|))))
+    (t (error "unreachable"))))
+
+(defun |foldr-38| (|f-16| |init-17| |?x₀-18|)
+  (case (|List/tag| |?x₀-18|)
+    (0
+      |init-17|)
+    (1
+      (let* ((|f-19| (|Cons/f0| |?x₀-18|))
+             (|f-20| (|Cons/f1| |?x₀-18|)))
+         (let* ((|app-21| (|foldr-38| |f-16| |init-17| |f-20|)))
+            (gapply2 |f-16| |f-19| |app-21|))))
+    (t (error "unreachable"))))
+
+(defun |fn-39| (|?x₀-24| |?x₁-25|)
+  (%int+ |?x₀-24| |?x₁-25|))
+
+(defun |fn-40| (|?x₀-29|)
+  (%int+ |?x₀-29| 1))
+
+(defparameter |i_Functor_0-2|
+  (%clos (function |fn-37|) 2))
+
+(defparameter |main-14|
+  (let* ((|fn-23| (%clos (function |fn-39|) 2))
+         (|fn-28| (%clos (function |fn-40|) 1))
+         (|con-31| (|mk/Nil|))
+         (|con-32| (|mk/Cons| 3 |con-31|))
+         (|con-33| (|mk/Cons| 2 |con-32|))
+         (|con-34| (|mk/Cons| 1 |con-33|))
+         (|app-35| (|fn-37| |fn-28| |con-34|)))
+     (|foldr-38| |fn-23| 0 |app-35|)))
