examples/typeclass0.tig.lisp
@@ -2,9 +2,11 @@
 
 let i_Functor_0 : Functor (Λa. a) = Functor@(Λa. a) Λ a₁ b. fun f : a₁ → b => f
 
-let main : Int =
-  let rd_Functor_0 : Functor (Λα. Int) = i_Functor_0
-  in rd_Functor_0[0, fmap]@(Λα. Int) fun ?x₀ : Int => add 1 ?x₀ 2
+let main : Int × Int =
+  let rd_Functor_0 : Functor (Λa. a) = i_Functor_0
+  in let x : Int = rd_Functor_0[0, fmap]@(Λa. a) fun ?x₀ : Int => add 1 ?x₀ 2
+     and y : Int = rd_Functor_0[0, fmap]@(Λa. a) fun _ : Bool => 1 true
+     in ⟨x, y⟩
 ;; == Runtime ==
 (load "runtime.lisp")
 
@@ -40,22 +42,30 @@ let main : Int =
     (%apply-slow c (list a1 a2))))
 
 ; ftype
-(declaim (ftype (function (clos) clos) |fn-12|))
+(declaim (ftype (function (clos) clos) |fn-17|))
 
-(declaim (ftype (function (integer) integer) |fn-13|))
+(declaim (ftype (function (integer) integer) |fn-18|))
 
-(declaim (type integer |main-6|))
+(declaim (ftype (function (boolean) integer) |fn-19|))
+
+(declaim (type cons |main-6|))
 
 ; body
-(defun |fn-12| (|f-4|)
+(defun |fn-17| (|f-4|)
   |f-4|)
 
-(defun |fn-13| (|?x₀-9|)
+(defun |fn-18| (|?x₀-9|)
   (%int+ 1 |?x₀-9|))
 
+(defun |fn-19| (|_-14|)
+  1)
+
 (defparameter |i_Functor_0-2|
-  (%clos (function |fn-12|) 1))
+  (%clos (function |fn-17|) 1))
 
 (defparameter |main-6|
-  (let* ((|fn-8| (%clos (function |fn-13|) 1)))
-     (gapply2 |i_Functor_0-2| |fn-8| 2)))
+  (let* ((|fn-8| (%clos (function |fn-18|) 1))
+         (|app-11| (gapply2 |i_Functor_0-2| |fn-8| 2))
+         (|fn-13| (%clos (function |fn-19|) 1))
+         (|app-15| (gapply2 |i_Functor_0-2| |fn-13| t)))
+     (cons |app-11| |app-15|)))
