tests/cases/impred/imp5.tig.lisp
@@ -1,0 +1,97 @@
+;; == System F IR ==
+
+let id : ∀α, α → α = Λ α. fun x : α => x
+
+let head : ∀α, List (α → α) → α → α =
+  Λ α.
+    fun l : List (α → α) =>
+      match l with
+      | Cons x _ => x
+      | Nil => id@α
+
+let ids : ∀α, List (α → α) = Λ α. Cons@(α → α) id@α Nil@(α → α)
+
+let run : (∀s, s → s) → Int = fun f : ∀s, s → s => f 1
+
+let main : Int = run (head@?m.10 ids@?m.10)
+;; == Runtime ==
+(load "runtime.lisp")
+
+;; == Linked Lisp Source ==
+(load "ffi.lisp")
+
+;; == Common Lisp ==
+
+; Prelude
+(declaim (optimize (speed 3) (safety 0) (debug 0)))
+(load "runtime.lisp")
+(defstruct (clos (:constructor %clos (fn arity)))
+  (fn #'identity :type function)
+  (arity 0 :type fixnum))
+(defun %apply-slow (c args)
+  (declare (type list args))
+  (let ((n (length args)) (k (clos-arity c)))
+    (cond
+      ((= n k) (apply (clos-fn c) args))
+      ((< n k) (%clos (lambda (&rest more)
+                        (apply (clos-fn c)
+                               (append args more)))
+                      (- k n)))
+      (t (%apply-slow (apply (clos-fn c)
+                             (subseq args 0 k))
+                      (nthcdr k args))))))
+
+
+; struct
+(defstruct (|List| (:conc-name |List/|) (:constructor nil) (:predicate nil))
+  (|tag| 0 :type (unsigned-byte 8)))
+
+(defstruct (|c/Nil| (:include |List| (|tag| 0))
+  (:conc-name |Nil/|)
+  (:constructor |mk/Nil| ())
+  (:predicate |Nil?|)))
+
+(defstruct (|c/Cons| (:include |List| (|tag| 1))
+  (:conc-name |Cons/|)
+  (:constructor |mk/Cons| (|f0| |f1|))
+  (:predicate |Cons?|))
+  (|f0| nil)
+  (|f1| nil))
+
+; gapply
+(defun gapply1 (c a1)
+  (if (eql (clos-arity c) 1)
+    (funcall (clos-fn c) a1)
+    (%apply-slow c (list a1))))
+
+; ftype
+(declaim (ftype (function (|List|) clos) |head-4|))
+
+(declaim (type |List| |ids-8|))
+
+(declaim (ftype (function (clos) integer) |run-11|))
+
+(declaim (type integer |main-14|))
+
+; body
+(defun |id-2| (|x-3|)
+  |x-3|)
+
+(defun |head-4| (|l-5|)
+  (case (|List/tag| |l-5|)
+    (0
+      (%clos (function |id-2|) 1))
+    (1
+      (let* ((|f-6| (|Cons/f0| |l-5|))
+             (|f-7| (|Cons/f1| |l-5|)))
+         |f-6|))
+    (t (error "unreachable"))))
+
+(defun |run-11| (|f-12|)
+  (gapply1 |f-12| 1))
+
+(defparameter |ids-8|
+  (let* ((|con-9| (|mk/Nil|))) (|mk/Cons| (%clos (function |id-2|) 1) |con-9|)))
+
+(defparameter |main-14|
+  (let* ((|app-15| (|head-4| |ids-8|))) (|run-11| |app-15|)))
