Tigris/lexing.lean
@@ -16,19 +16,20 @@ def String.isLowerInit (s : String) : Bool :=
 
 namespace Lexing open Parser Parser.Char
 @[inline] def _root_.Char.isGreek (n : Char) : Bool := n.toNat >= 0x0370 && n.toNat <= 0x3FF
+@[inline] def _root_.Char.isSubscript (n : Char) : Bool := n.toNat >= 0x2070 && n.toNat <= 0x209F
 
 def alphanum' [Parser.Stream σ Char] [Parser.Error ε σ Char] [Monad m]
   : ParserT ε σ Char m Char :=
   withErrorMessage "expected letter or digit character or \'" do
-    tokenFilter fun c => c.isAlphanum || c.isGreek || c == '\'' || c == '_' || c == '!' || c == '?'
+    tokenFilter fun c => c.isAlphanum || c.isGreek || c.isSubscript || c == '\'' || c == '_' || c == '!' || c == '?'
 def alphanum'' [Parser.Stream σ Char] [Parser.Error ε σ Char] [Monad m]
   : ParserT ε σ Char m Char :=
   withErrorMessage "expected letter or digit character or \'" do
-    tokenFilter fun c => c.isAlphanum || c.isGreek || c == '\'' || c == '_' || c == '!' || c == '?' || c == '-' || c == '/'
+    tokenFilter fun c => c.isAlphanum || c.isGreek || c.isSubscript || c == '\'' || c == '_' || c == '!' || c == '?' || c == '-' || c == '/'
 def alpha' [Parser.Stream σ Char] [Parser.Error ε σ Char] [Monad m]
   : ParserT ε σ Char m Char :=
   withErrorMessage "expected alphabetic character" do
-    tokenFilter fun c => c.isGreek || if c >= 'a' then c <= 'z' else c == '_' || c >= 'A' && c <= 'Z'
+    tokenFilter fun c => c.isSubscript || c.isGreek || if c >= 'a' then c <= 'z' else c == '_' || c >= 'A' && c <= 'Z'
 def oneOf [Parser.Stream σ Char] [Parser.Error ε σ Char] [Monad m] (l : List Char)
   : ParserT ε σ Char m Char := withBacktracking $ withErrorMessage s!"expected one of {l}" $ tokenFilter (· ∈ l)
 
